\subsection{Recap of the $\cup $ and $\cap $ products}
\label{sec:recap-cap-cup-product}

Let $(X,A,B)$ be an excisive triad.
Then, the cup product is a natural morphism
 \[
  \cup \colon H^k(X,A;R) \tensor _R H^l(X,b;R)
  \xrightarrow{} H^{k+l}(X,A\cup B;R) 
\]
that satisfies
\begin{enumerate}[h]
  \item $x\cup y = (-1)^{\abs{x} \cdot \abs{y} } y\cup x$
  \item $(x\cup y)\cup z = x\cup (y\cup z)$ 
  \item $δ(\varphi \cup \psi )
    =
    (δ \varphi )\cup \psi + (-1)^{\abs{\varphi } } \varphi  \cup (δ\psi )$ on chain level.
\end{enumerate}
\todo{different sign convention?}

The cap product is defined by
\[
  \varphi ^k \cap σ^n = \varphi (\frestriction{σ}{[n-k,\ldots,n} \frestriction{σ}{0,\dotsc, n-k}
\]
such that
\[
  \cap \colon H^k(X,A;R)\tensor_R H_{k+l}(X,A\cup B;R)
  \to 
  H_l(X,B;R)
\]
It is natural in the sense that
\[
  x \cap f_*α = f_*(f^*x \cap  α)
\] 
\todo{Hatcher: right modules}
\begin{enumerate}[h]
  \item We have $x \cap (y \cap α) = (x\cup y) \cap α$
  \item On chain level, we have
    \[
      \partial (\varphi  \cap σ) = \varphi  \cap (\partial σ) + (-1)^{\abs{\varphi } \abs{σ} } (δ\varphi )\cap σ
    \]
  \item Let $x = [\varphi ] \in H^k(X;R)$ and $α = [σ] \in H_k(X;R)$,
    then
    \[
      \left< x,α \right> =\varphi (σ)\in R
    .\]
    This yields the cap product if $R$ is connected. 
    Thus
    \[
      \left< x, y \cap α \right>  = \left< x\cup y, α \right> 
    .\] 
\end{enumerate}
